\documentclass{article}
\usepackage[T2A, T1]{fontenc}
\usepackage{fancyhdr}
\usepackage{setspace}
\usepackage{titlesec}
\usepackage{amsmath}
\usepackage{amssymb}
\usepackage{amsthm}
\usepackage[english, russian]{babel}

\setlength{\parindent}{0pt}
\setlength{\parskip}{0pt}

\theoremstyle{plain} \newtheorem*{theorem*}{Теорема}
\theoremstyle{plain} \newtheorem{theorem}{Теорема}[section]
% \theoremstyle{remark} \newtheorem{definition}{Definition}[section]
% \theoremstyle{remark} \newtheorem{notation}{Notation}[section]
\theoremstyle{definition} \newtheorem*{corollary*}{Следствие}
\theoremstyle{definition} \newtheorem{corollary}{Следствие}[section]
\theoremstyle{remark} \newtheorem*{example*}{Пример}


\begin{document}

\abovedisplayskip=0pt
\belowdisplayskip=9pt
\abovedisplayshortskip=0pt
\belowdisplayshortskip=12pt


\begin{equation}
    \ddot{x} + a(t)\dot{x} + b(t)x = f(t)
\end{equation}

$a(t)$, $b(t)$, $f(t)$, $t_0 \le t \le t_1$
$x(t)$

\begin{gather}
    \begin{split}
        \dot{x}(t_0) - \alpha_0 x(t_0) = \alpha_1, \\
        \dot{x}(t_1) - \beta_0 x(t_1) = \beta_1,
    \end{split}
\end{gather}

$\alpha_0, \alpha_1, \beta_0, \beta_1$,
$x(t)$, $\dot{x}(t)$, $t = t_0$, $t = t_1$,

\begin{example*}
    This is example

    \begin{equation}
        \ddot{x} + x = 0
    \end{equation}

    \begin{equation}
        x = c_1 \cos(t) + c_2 \sin(t)
    \end{equation}

    \begin{align}
        &\dot{x}(0) = 0, &\dot{x}(1) = 1; \\
        &\dot{x}(0) = 0, &\dot{x}(\pi) = 1; \\
        &\dot{x}(0) = 0, &\dot{x}(\pi) = 0;
    \end{align}

    \begin{equation*}
        c_1 = - \frac{1}{\sin(t)}, \ \ \ \ \ \
        c_2 = 0,
    \end{equation*}

    \begin{equation*}
        1 = -c_1 \sin(\pi) = 0
    \end{equation*}

    \begin{equation*}
        x = c_1 \cos(t)
    \end{equation*}

    $c_1$,

\end{example*}

Solving boundary problem using Green's function

\begin{equation}
    \ddot{x} + a(t)\dot{x} + b(t)x = f(t)
\end{equation}

\begin{gather}
\begin{split}
    & \alpha_0 \dot{x}(t_0) + \alpha_1 x(t_0) = 0
    \ \ \ \ (\alpha^2_0 + \alpha^2_1 > 0) \\
    & \beta_0 \dot{x}(t_1) + \beta_1 x(t_1) = 0
    \ \ \ \ (\beta^2_0 + \beta^2_1 > 0)
\end{split}
\end{gather}

$x = x_1(t)$,

\begin{equation}
    \ddot{x} + a(t) \dot{x} + b(t)x = 0
\end{equation}

\begin{equation*}
    \alpha_0 \dot{x_1}(t_0) + \alpha_1 x_1(t_0) = 0
\end{equation*}

$x = x_2(t)$

\begin{equation*}
    \beta_0 \dot{x_2}(t_1) + \beta_1 x_2(t_1) = 0
\end{equation*}

$x_1(t)$,
$c$,
$x = cx_1(t)$,
$x_2(t)$

\begin{gather}
    \begin{split}
    \beta_0 \dot{x_1}(t_1) + \beta_1 x_1(t_1) \ne 0 \\
    \alpha_0 \dot{x_2}(t_0) + \alpha_1 x_2(t_0) \ne 0
    \end{split}
\end{gather}

$x = x_1(t)$,
$x = x_2(t)$,
$x(t)$,

\begin{equation}
    x(t) = c_1(t) x_1(t) + c_2(t) x_2(t)
\end{equation}

$\dot{c}_1(t)$,
$\dot{c}_2(t)$,

\begin{align*}
    & \dot{c}_1(t) x_1(t) + \dot{c}_2(t) x_2(t) = 0 \\
    & \dot{c}_1(t) \dot{x}_1(t) + \dot{c}_2(t) \dot{x}_2(t) = f(t)
\end{align*}

\begin{gather}
    \begin{split}
        & \dot{c}_1(t) = - \frac{x_2(t)f(t)}{w(t)}, \\
        & \dot{c}_2(t) = \frac{x_1(t)f(t)}{w(t)},
    \end{split}
\end{gather}

where

\begin{equation*}
    w(t) =
    \begin{vmatrix}
        x_1(t) & x_2(t) \\
        \dot{x}_1(t) & \dot{x}_2(t)
    \end{vmatrix}
    \ne 0
\end{equation*}

$x_1(t)$,
$x_2(t)$,

\begin{align*}
    & c_1(t) = - \int^t_{t_1} \frac{x_2(s)f(s)}{w(s)} ds + \gamma_1
    = \int^{t_1}_t \frac{x_2(s)f(s)}{w(s)} ds + \gamma_1, \\
    & c_2(t) = \int^t_{t_0} \frac{x_1(s)f(s)}{w(s)} ds + \gamma_2
\end{align*}

where $\gamma_1$, $\gamma_2$,
$c_1(t)$, $c_2(t)$

\begin{equation}
    x(t) =
    x_1(t)\int^{t_1}_t \frac{x_2(s)f(s)}{w(s)} ds +
    x_2(t)\int^t_{t_0} \frac{x_1(s)f(s)}{w(s)} ds
    + \gamma_1 x_1(t)
    + \gamma_2 x_2(t)
\end{equation}

$t$,

\begin{equation}
    \dot{x}(t) =
    \dot{x}_1(t)\int^{t_1}_t \frac{x_2(s)f(s)}{w(s)} ds +
    \dot{x}_2(t)\int^t_{t_0} \frac{x_1(s)f(s)}{w(s)} ds
    + \gamma_1 \dot{x}_1(t)
    + \gamma_2 \dot{x}_2(t)
\end{equation}

($\alpha_0 \dot{x}_1(t_0) + \alpha_1 x_1(t_0) = 0$)

\begin{align*}
    & 0 =
    (\alpha_0 \dot{x}_1(t_0) + \alpha_1 x_1(t_0))
    \int^{t_1}_t \frac{x_2(s)f(s)}{w(s)} ds +
    \gamma_1
    (\alpha_0 \dot{x}_1(t_0) + \alpha_1 x_1(t_0)) + \\
    & + \gamma_2(\alpha_0 \dot{x}_2(t_0) + \alpha_1 x_2(t_0)) =
    \gamma_2(\alpha_0 \dot{x}_2(t_0) + \alpha_1 x_2(t_0))
\end{align*}

$\gamma_2 = 0$,
$\gamma_1 = 0$,

\begin{equation*}
    x(t) =
    x_1(t)\int^{t_1}_t \frac{x_2(s)f(s)}{w(s)} ds +
    x_2(t)\int^t_{t_0} \frac{x_1(s)f(s)}{w(s)} ds
\end{equation*}

or

\begin{equation}
    x(t) = \int^{t_1}_{t_0} G(t, s) f(s) ds
\end{equation}

\begin{equation}
    G(t,s) =
    \begin{cases}
        \frac{x_1(s) x_2(t)}{w(s)} , &t_0 \le s \le t,\\
        \frac{x_1(t) x_2(s)}{w(s)} , &t \le s \le t_1,\\
        \frac{x_1(s) x_2(t)}{w(s)} , &t_0 \le t \le s,\\
        \frac{x_1(t) x_2(s)}{w(s)} , &s \le t \le t_1,\\
    \end{cases}
\end{equation}

$G(t,s)$,
$f(t)$,
$x_1(t)$,
$x_2(t)$,
$G(t,s)$,

\begin{enumerate}
    \item $t \ne s$ $G(t,s)$;
    \item $t = t_0$ $t = t_1$ $G(t,s)$;
    \item $t = s$ $G(t,s)$;
    \item $t = s$ $G'_t(t,s)$ :
        \begin{equation*}
            G'_t \vert_{t = s + 0} - G'_t \vert_{t = s - 0} = 1
        \end{equation*}
\end{enumerate}

\begin{equation*}
    G'_t =
    \begin{cases}
        \frac{\dot{x}_1(t) x_2(s)}{w(s)}, &t_0 \le t \le s, \\
        \frac{x_1(s) \dot{x}_2(t)}{w(s)}, &s \le t \le t_1,
    \end{cases}
\end{equation*}

\begin{equation*}
    G'_t \vert_{t = s + 0} - G'_t \vert_{t = s - 0} =
    \frac{x_1(s) \dot{x}_2(s) - \dot{x}_1(s) x_2(s)}{w(s)} = 1.
\end{equation*}

$G(t,s)$,
$f(t)$,


\end{document}
